Low-level Merkle tree: separated high and low-level impls

examples/low-level/merkletree/MerkleTree.Low.fst
@@ -1,5 +1,7 @@
 module MerkleTree.Low
 
+open MerkleTree.High
+
 open FStar.All
 open FStar.Mul
 open LowStar.Modifies
@@ -12,22 +14,11 @@ module HST = FStar.HyperStack.ST
 module B = LowStar.Buffer
 module S = FStar.Seq
 
-let root = Monotonic.HyperHeap.root
+module High = MerkleTree.High
 
-assume type elem: eqtype u#0
-assume type hash: eqtype u#0
-assume val elem_init: elem
-assume val hash_init: hash
+let root = Monotonic.HyperHeap.root
 let elem_buf = B.buffer elem
 let hash_buf = B.buffer hash
-let elem_seq = S.seq elem
-let hash_seq = S.seq hash
-
-assume val hash_from_elem: elem -> Tot hash
-
-assume val hash_from_hashes: hash -> hash -> Tot hash
-assume val hash_init_idem: 
-  h:hash -> Lemma (hash_from_hashes h hash_init = h)
 
 // This number says that the maximum number of values is (2^32 - 1)
 unfold let max_nelts_sz = 32
@@ -44,68 +35,23 @@ let rec seq_map #a #b f s =
   if S.length s = 0 then S.empty
   else S.cons (f (S.head s)) (seq_map f (S.tail s))
 
-val seq_map_create:
-  #a:Type -> #b:Type -> f: (a -> b) -> 
-  len:nat -> ia:a ->
-  Lemma (seq_map f (S.create len ia) == S.create len (f ia))
-let seq_map_create #a #b f len ia =
-  S.lemma_eq_intro (seq_map f (S.create len ia)) (S.create len (f ia))
+// val seq_map_create:
+//   #a:Type -> #b:Type -> f: (a -> b) -> 
+//   len:nat -> ia:a ->
+//   Lemma (seq_map f (S.create len ia) == S.create len (f ia))
+// let seq_map_create #a #b f len ia =
+//   S.lemma_eq_elim (seq_map f (S.create len ia)) (S.create len (f ia))
 
 /// Allocation by power of two
-
-// TODO: optimize using bit manipulation
-val is_pow2: nat -> Tot bool
-let rec is_pow2 n =
-  if n = 0 then false
-  else if n = 1 then true
-  else (n % 2 = 0 && is_pow2 (n / 2))
-
-val pow2_is_pow2:
-  n:nat ->
-  Lemma (is_pow2 (pow2 n))
-	[SMTPat (is_pow2 (pow2 n))]
-let rec pow2_is_pow2 n =
-  if n = 0 then ()
-  else pow2_is_pow2 (n - 1)
 
 val alloc_sz_lg:
   nelts:nat{nelts > 0} -> 
   GTot (sz:nat{sz > 0 && pow2 (sz - 1) <= nelts && nelts < pow2 sz})
-let rec alloc_sz_lg nelts =
-  if nelts = 1 then 1
-  else 1 + alloc_sz_lg (nelts / 2)
+let rec alloc_sz_lg nelts = pow2_floor nelts + 1
 
 unfold val alloc_sz: nelts:nat{nelts > 0} -> GTot nat
 unfold let alloc_sz nelts =
   pow2 (alloc_sz_lg nelts) - 1
-
-val pow2_interval_unique:
-  n:nat -> sz1:nat{sz1 > 0} -> sz2:nat{sz2 > 0} ->
-  Lemma (requires (pow2 (sz1 - 1) <= n && n < pow2 sz1 &&
-		  pow2 (sz2 - 1) <= n && n < pow2 sz2))
-	(ensures (sz1 = sz2))
-let pow2_interval_unique n sz1 sz2 =
-  if sz1 > sz2 
-  then Math.Lemmas.pow2_le_compat (sz1 - 1) sz2
-  else if sz1 < sz2
-  then Math.Lemmas.pow2_le_compat (sz2 - 1) sz1
-  else ()
-
-val alloc_sz_lg_inv:
-  nelts:nat -> sz:nat{sz > 0} ->
-  Lemma (requires (pow2 (sz - 1) <= nelts && nelts < pow2 sz))
-	(ensures (alloc_sz_lg nelts = sz))
-let alloc_sz_lg_inv nelts sz =
-  pow2_interval_unique nelts sz (alloc_sz_lg nelts)
-
-val alloc_sz_lg_pow2:
-  nelts:nat ->
-  Lemma (requires (is_pow2 nelts))
-	(ensures (nelts = pow2 (alloc_sz_lg nelts - 1)))
-let rec alloc_sz_lg_pow2 nelts =
-  if nelts = 1 then ()
-  else if nelts % 2 = 0 then alloc_sz_lg_pow2 (nelts / 2)
-  else ()
 
 val alloc_sz_lg_pow2_inc:
   nelts:nat{nelts > 0} ->
@@ -143,79 +89,42 @@ noeq type merkle_tree =
 
 let mtree_ptr = B.pointer merkle_tree
 
-/// Invariants between internal roots and values
-
-val merkle_root_of_pow2:
-  #nelts:nat{is_pow2 nelts} -> vs:hash_seq{S.length vs = nelts} -> 
-  GTot hash
-let rec merkle_root_of_pow2 #nelts vs =
-  if nelts = 1 then S.index vs 0
-  else 
-    let lrt = merkle_root_of_pow2 #(nelts / 2) (S.slice vs 0 (nelts / 2)) in
-    let rrt = merkle_root_of_pow2 #(nelts / 2) (S.slice vs (nelts / 2) nelts) in
-    hash_from_hashes lrt rrt
-
-val pow2_floor: 
-  n:nat{n > 0} -> GTot (p:nat{pow2 p <= n && n < pow2 (p + 1)})
-let rec pow2_floor n =
-  if n = 1 then 0 else 1 + pow2_floor (n / 2)
-
-val num_iroots_of: 
-  nelts_sz:nat -> nelts:nat{nelts < pow2 nelts_sz} -> 
-  GTot (nirs:nat{nirs <= nelts_sz})
-let rec num_iroots_of nelts_max_lg nelts =
+val num_iroots_of_bound: 
+  #nelts_sz:nat -> nelts:nat{nelts < pow2 nelts_sz} -> 
+  GTot (nirs:nat{nirs = num_iroots_of nelts && nirs <= nelts_sz})
+let rec num_iroots_of_bound #nelts_sz nelts =
   if nelts = 0 then 0
-  else 1 + num_iroots_of (nelts_max_lg - 1) (nelts - pow2 (pow2_floor nelts))
+  else 1 + num_iroots_of_bound #(nelts_sz - 1) (nelts - pow2 (pow2_floor nelts))
 
-val iroots_of_hashes:
-  nelts_sz:nat -> nelts:nat{nelts < pow2 nelts_sz} -> 
-  hs:hash_seq{S.length hs = nelts} ->
-  GTot (iroots:hash_seq{S.length iroots = num_iroots_of nelts_sz nelts})
-let rec iroots_of_hashes nelts_sz nelts hs =
-  if nelts = 0 then hs
-  else S.cons (merkle_root_of_pow2 #(pow2 (pow2_floor nelts))
-				   (S.slice hs 0 (pow2 (pow2_floor nelts))))
-	      (iroots_of_hashes (nelts_sz - 1) (nelts - (pow2 (pow2_floor nelts)))
-				(S.slice hs (pow2 (pow2_floor nelts)) nelts))
+val merkle_tree_lift: HS.mem -> merkle_tree -> GTot (High.merkle_tree)
+let merkle_tree_lift h mt =
+  High.MT (MT?.nelts mt) 
+	  (S.slice (B.as_seq h (MT?.values mt)) 0 (MT?.nelts mt))
+	  (S.slice (B.as_seq h (MT?.iroots mt)) 
+	    0 (num_iroots_of_bound #max_nelts_sz (MT?.nelts mt)))
 
-unfold val iroots_of: 
-  nelts_sz:nat -> nelts:nat{nelts < pow2 nelts_sz} -> 
-  es:elem_seq{S.length es = nelts} -> GTot hash_seq
-unfold let iroots_of nelts_sz nelts vs =
-  iroots_of_hashes nelts_sz nelts (seq_map hash_from_elem vs)
-
-unfold val merkle_tree_elems_wf:
-  nelts:nat{nelts > 0 && nelts < pow2 max_nelts_sz} -> 
-  values:elem_seq{S.length values = nelts} ->
-  iroots:hash_seq{S.length iroots = num_iroots_of max_nelts_sz nelts} ->
-  GTot bool
-unfold let merkle_tree_elems_wf nelts values iroots =
-  iroots_of max_nelts_sz nelts values = iroots
+/// Low-level well-formedness
 
 unfold val merkle_tree_wf: HS.mem -> merkle_tree -> GTot Type0
 unfold let merkle_tree_wf h mt =
-  B.live h (MT?.values mt) /\ B.live h (MT?.iroots mt) /\
-  merkle_tree_elems_wf 
-    (MT?.nelts mt) 
-    (S.slice (B.as_seq h (MT?.values mt)) 0 (MT?.nelts mt))
-    (S.slice (B.as_seq h (MT?.iroots mt)) 0 (num_iroots_of max_nelts_sz (MT?.nelts mt)))
+  B.live h (MT?.values mt) /\ B.freeable (MT?.values mt) /\ 
+  B.live h (MT?.iroots mt) /\
+  B.disjoint (MT?.values mt) (MT?.iroots mt) /\
+  High.merkle_tree_wf (merkle_tree_lift h mt)
 
 /// Initialization
 
 val create_merkle_tree: unit -> 
   HST.ST merkle_tree
 	 (requires (fun _ -> true))
-	 (ensures (fun h0 mt h1 -> 
-	   B.freeable (MT?.values mt) /\ 
-	   B.disjoint (MT?.values mt) (MT?.iroots mt) /\
-	   merkle_tree_wf h1 mt))
+	 (ensures (fun h0 mt h1 -> merkle_tree_wf h1 mt))
 let create_merkle_tree _ = 
   let values = B.malloc root elem_init 1ul in
   let hh0 = HST.get () in
   let iroots = B.malloc root (hash_from_elem elem_init) (UInt32.uint_to_t max_nelts_sz) in
   let hh1 = HST.get () in
   B.live_unused_in_disjoint hh0 values iroots;
-  S.lemma_eq_intro (iroots_of max_nelts_sz 1 (S.slice (B.as_seq hh1 values) 0 1))
+  S.lemma_eq_intro (iroots_of 1 (S.slice (B.as_seq hh1 values) 0 1))
   		   (S.slice (B.as_seq hh1 iroots) 0 1);
   MT 1 values iroots
 
@@ -228,23 +137,13 @@ let create_merkle_tree _ =
 val mt_is_full: merkle_tree -> Tot bool
 let mt_is_full mt = MT?.nelts mt >= pow2 max_nelts_sz - 1
 
-unfold val insert_nelts: 
+val insert_nelts: 
   nelts:nat{nelts < pow2 max_nelts_sz - 1} ->
-  Tot (inelts:nat{inelts < pow2 max_nelts_sz})
-unfold let insert_nelts nelts =
+  Tot (inelts:nat{
+      inelts = High.insert_nelts nelts && 
+      inelts < pow2 max_nelts_sz})
+let insert_nelts nelts =
   nelts + 1
-
-val pow2_lt_le:
-  n:nat -> p:nat{p > 0} ->
-  Lemma (requires (is_pow2 n && n < pow2 p))
-	(ensures (n <= pow2 (p - 1)))
-let rec pow2_lt_le n p =
-  if n = 1 then ()
-  else pow2_lt_le (n / 2) (p - 1)
-
-val insert_values_seq: elem_seq -> elem -> GTot elem_seq
-let insert_values_seq vs nv =
-  S.append vs (S.create 1 nv)
 
 val insert_values:
   nelts:nat{nelts > 0 && nelts < pow2 max_nelts_sz - 1} -> 
@@ -255,8 +154,8 @@ val insert_values:
 	 (ensures (fun h0 nvs h1 -> 
 	   B.live h1 nvs /\ B.freeable nvs /\
 	   S.slice (B.as_seq h1 nvs) 0 (insert_nelts nelts) ==
-	   insert_values_seq (S.slice (B.as_seq h0 vs) 0 nelts) e))
-#set-options "--z3rlimit 10"
+	   High.insert_values (S.slice (B.as_seq h0 vs) 0 nelts) e))
+#set-options "--z3rlimit 20"
 let insert_values nelts vs e =
   if is_pow2 (nelts + 1)
   then (let hh0 = HST.get () in
@@ -271,8 +170,8 @@ let insert_values nelts vs e =
 
        B.upd nvs (UInt32.uint_to_t nelts) e;
        let hh1 = HST.get () in
-       S.lemma_eq_intro (S.slice (B.as_seq hh1 nvs) 0 (insert_nelts nelts))
-       			(insert_values_seq (S.slice (B.as_seq hh0 vs) 0 nelts) e);
+       S.lemma_eq_elim (S.slice (B.as_seq hh1 nvs) 0 (insert_nelts nelts))
+       		       (High.insert_values (S.slice (B.as_seq hh0 vs) 0 nelts) e);
 
        // TODO: should be able to prove that `nvs` is not affected after `B.free`
        // there might be a relation among `B.disjoint`, `B.free`, and `B.live`
@@ -284,19 +183,11 @@ let insert_values nelts vs e =
   else (let hh0 = HST.get () in
        B.upd vs (UInt32.uint_to_t nelts) e; 
        let hh1 = HST.get () in
-       S.lemma_eq_intro (S.slice (B.as_seq hh1 vs) 0 (insert_nelts nelts))
-       			(insert_values_seq (S.slice (B.as_seq hh0 vs) 0 nelts) e);
+       S.lemma_eq_elim (S.slice (B.as_seq hh1 vs) 0 (insert_nelts nelts))
+       		       (High.insert_values (S.slice (B.as_seq hh0 vs) 0 nelts) e);
 
        alloc_sz_lg_not_pow2_inc nelts;
        vs)
-
-val insert_iroots_seq:
-  nelts:nat{nelts > 0 && nelts < pow2 max_nelts_sz - 1} ->
-  irs:hash_seq{S.length irs = max_nelts_sz} ->
-  nv:elem ->
-  GTot (iirs:hash_seq{S.length iirs = max_nelts_sz})
-let insert_iroots_seq nirs irs nv =
-  admit ()
 
 val insert_iroots:
   nelts:nat{nelts > 0 && nelts < pow2 max_nelts_sz - 1} ->
@@ -306,79 +197,27 @@ val insert_iroots:
 	 (requires (fun h0 -> B.live h0 irs))
 	 (ensures (fun h0 _ h1 -> 
 	   modifies (loc_buffer irs) h0 h1 /\
-	   insert_iroots_seq nelts (B.as_seq h0 irs) nv =
-	   B.as_seq h1 irs))
+	   S.slice (B.as_seq h1 irs) 0 (num_iroots_of_bound #max_nelts_sz (insert_nelts nelts)) ==
+	   High.insert_iroots 
+	     nelts (S.slice (B.as_seq h0 irs) 0 (num_iroots_of_bound #max_nelts_sz nelts)) 
+	     (hash_from_elem nv)))
 let rec insert_iroots nirs irs nv =
-  admit ()
-
-val insert_iroots_ok:
-  nelts:nat{nelts > 0 && nelts < pow2 max_nelts_sz - 1} ->
-  values:elem_seq{S.length values = nelts} ->
-  irs:hash_seq{S.length irs = max_nelts_sz} -> nv:elem ->
-  Lemma (requires (merkle_tree_elems_wf nelts (S.slice values 0 nelts) 
-					(S.slice irs 0 (num_iroots_of max_nelts_sz nelts))))
-	(ensures (merkle_tree_elems_wf (insert_nelts nelts)
-				       (insert_values_seq values nv)
-				       (S.slice irs 0 (num_iroots_of max_nelts_sz (insert_nelts nelts)))))
-let rec insert_iroots_ok nelts values irs nv =
   admit ()
 
 val insert: 
   mt:merkle_tree -> e:elem -> 
   HST.ST merkle_tree
-	 (requires (fun h0 -> 
-	   MT?.nelts mt < pow2 max_nelts_sz - 1 /\
-	   B.disjoint (MT?.values mt) (MT?.iroots mt) /\
-	   B.live h0 (MT?.values mt) /\ B.freeable (MT?.values mt) /\
-	   B.live h0 (MT?.iroots mt) /\ B.freeable (MT?.iroots mt) /\
-	   ~ (mt_is_full mt) /\
-	   merkle_tree_wf h0 mt))
-	 (ensures (fun h0 nmt h1 -> merkle_tree_wf h1 nmt))
+	 (requires (fun h0 -> merkle_tree_wf h0 mt /\ ~ (mt_is_full mt)))
+	 (ensures (fun h0 nmt h1 ->
+	   merkle_tree_wf h1 nmt /\
+	   High.insert (merkle_tree_lift h0 mt) e == merkle_tree_lift h1 nmt))
 let insert mt e =
   let nnelts = insert_nelts (MT?.nelts mt) in
   let niroots = insert_iroots (MT?.nelts mt) (MT?.iroots mt) e; MT?.iroots mt in
   let nvalues = insert_values (MT?.nelts mt) (MT?.values mt) e in
-  assert (nnelts > 0 && nnelts < pow2 max_nelts_sz);
-  assert (B.length nvalues = alloc_sz nnelts);
-  assert (B.length niroots = max_nelts_sz);
   admit () // MT nnelts nvalues niroots
 
 /// Getting the Merkle root
-
-val padding_to_pow2:
-  nelts:nat{nelts > 0} -> GTot (sz:nat{
-    if nelts = 1 then sz = 0
-    else sz > 0 && pow2 (sz - 1) < nelts && nelts <= pow2 sz})
-let rec padding_to_pow2 nelts =
-  if nelts = 1 then 0
-  else if nelts % 2 = 0 then 1 + padding_to_pow2 (nelts / 2)
-  else 1 + padding_to_pow2 ((nelts + 1) / 2)
-
-val pad_hashes_pow2:
-  vs:hash_seq{S.length vs > 0} -> 
-  GTot (pvs:hash_seq{
-    S.length pvs = pow2 (padding_to_pow2 (S.length vs)) && 
-    S.slice pvs 0 (S.length vs) = vs})
-let pad_hashes_pow2 vs =
-  let pad = S.create (pow2 (padding_to_pow2 (S.length vs)) - S.length vs) hash_init in
-  S.append_slices vs pad;
-  S.append vs pad
-
-val merkle_root_of_hashes: vs:hash_seq{S.length vs > 0} -> GTot hash
-let merkle_root_of_hashes vs =
-  merkle_root_of_pow2 #(pow2 (padding_to_pow2 (S.length vs))) 
-		      (pad_hashes_pow2 vs)
-
-val merkle_root_of_iroots_seq':
-  acc:hash ->
-  nirs:nat{nirs <= max_nelts_sz} ->
-  irs:hash_seq{S.length irs = max_nelts_sz} -> 
-  GTot hash (decreases nirs)
-let rec merkle_root_of_iroots_seq' acc nirs irs =
-  if nirs = 0 then acc
-  else merkle_root_of_iroots_seq'
-       (hash_from_hashes (S.index irs (nirs - 1)) acc)
-       (nirs - 1) irs
 
 val merkle_root_of_iroots':
   acc:hash ->
@@ -388,19 +227,13 @@ val merkle_root_of_iroots':
 	 (requires (fun h0 -> B.live h0 irs))
 	 (ensures (fun h0 hs h1 -> 
 	   h1 == h0 /\
-	   merkle_root_of_iroots_seq' acc nirs (B.as_seq h0 irs) = hs))
+	   High.merkle_root_of_iroots' acc (B.as_seq h0 irs) = hs))
 let rec merkle_root_of_iroots' acc nirs irs =
-  if nirs = 0 then acc
-  else merkle_root_of_iroots'
-       (hash_from_hashes (B.index irs (UInt32.uint_to_t (nirs - 1))) acc)
-       (nirs - 1) irs
-
-val merkle_root_of_iroots_seq:
-  nirs:nat{nirs <= max_nelts_sz} ->
-  irs:hash_seq{S.length irs = max_nelts_sz} -> 
-  GTot hash (decreases nirs)
-let rec merkle_root_of_iroots_seq nirs irs =
-  merkle_root_of_iroots_seq' hash_init nirs irs
+  // if nirs = 0 then acc
+  // else merkle_root_of_iroots'
+  //      (hash_from_hashes (B.index irs (UInt32.uint_to_t (nirs - 1))) acc)
+  //      (nirs - 1) irs
+  admit () // TODO: need to prove `High.merkle_root_of_iroots'`
 
 val merkle_root_of_iroots:
   nirs:nat{nirs <= max_nelts_sz} ->
@@ -409,15 +242,7 @@ val merkle_root_of_iroots:
 	 (requires (fun h0 -> B.live h0 irs))
 	 (ensures (fun h0 hs h1 -> 
 	   h1 == h0 /\
-	   merkle_root_of_iroots_seq nirs (B.as_seq h0 irs) = hs))
+	   High.merkle_root_of_iroots (B.as_seq h0 irs) = hs))
 let merkle_root_of_iroots nirs irs =
   merkle_root_of_iroots' hash_init nirs irs
-
-val merkle_root_of_iroots_ok:
-  h:HS.mem -> mt:merkle_tree ->
-  Lemma (requires (merkle_tree_wf h mt))
-	(ensures (merkle_root_of_iroots_seq (num_iroots_of max_nelts_sz (MT?.nelts mt)) (B.as_seq h (MT?.iroots mt)) =
-		 merkle_root_of_hashes (seq_map hash_from_elem (B.as_seq h (MT?.values mt)))))
-let merkle_root_of_iroots_ok h mt =
-  admit ()
 
