examples/low-level/merkletree/MerkleTree.High.fst
@@ -1,0 +1,260 @@
+module MerkleTree.High
+
+open FStar.All
+open FStar.Mul
+open FStar.Seq
+
+module List = FStar.List.Tot
+module S = FStar.Seq
+
+assume type elem: eqtype u#0
+assume type hash: eqtype u#0
+assume val elem_init: elem
+assume val hash_init: hash
+let elem_seq = S.seq elem
+let hash_seq = S.seq hash
+
+assume val hash_from_elem: elem -> Tot hash
+assume val hash_from_hashes: hash -> hash -> Tot hash
+assume val hash_init_idem: 
+  h:hash -> Lemma (hash_from_hashes h hash_init = h)
+
+/// Mapping sequences (why is it not in the library?)
+
+val seq_map:
+  #a:Type -> #b:Type -> f:(a -> b) -> s:S.seq a -> 
+  Tot (fs:S.seq b{
+    S.length fs = S.length s /\
+    (forall (i:nat{i < S.length fs}). S.index fs i == f (S.index s i))})
+    (decreases (S.length s))
+let rec seq_map #a #b f s =
+  if S.length s = 0 then S.empty
+  else S.cons (f (S.head s)) (seq_map f (S.tail s))
+
+/// Power of two
+
+// TODO: optimize using bit manipulation
+val is_pow2: nat -> Tot bool
+let rec is_pow2 n =
+  if n = 0 then false
+  else if n = 1 then true
+  else (n % 2 = 0 && is_pow2 (n / 2))
+
+val pow2_is_pow2:
+  n:nat ->
+  Lemma (is_pow2 (pow2 n))
+	[SMTPat (is_pow2 (pow2 n))]
+let rec pow2_is_pow2 n =
+  if n = 0 then ()
+  else pow2_is_pow2 (n - 1)
+
+val pow2_lt_le:
+  n:nat -> p:nat{p > 0} ->
+  Lemma (requires (is_pow2 n && n < pow2 p))
+	(ensures (n <= pow2 (p - 1)))
+let rec pow2_lt_le n p =
+  if n = 1 then ()
+  else pow2_lt_le (n / 2) (p - 1)
+
+val pow2_floor: 
+  n:nat{n > 0} -> GTot (p:nat{pow2 p <= n && n < pow2 (p + 1)})
+let rec pow2_floor n =
+  if n = 1 then 0 else 1 + pow2_floor (n / 2)
+
+val pow2_floor_pow2:
+  p:nat -> 
+  Lemma (pow2_floor (pow2 p) = p)
+	[SMTPat (pow2_floor (pow2 p))]
+let rec pow2_floor_pow2 p =
+  if p = 0 then ()
+  else pow2_floor_pow2 (p - 1)
+
+val pow2_floor_is_pow2:
+  n:nat ->
+  Lemma (requires (is_pow2 n))
+	(ensures (n = pow2 (pow2_floor n)))
+let rec pow2_floor_is_pow2 n =
+  if n = 1 then ()
+  else pow2_floor_is_pow2 (n / 2)
+
+val pow2_interval_unique:
+  n:nat -> p1:nat -> p2:nat ->
+  Lemma (requires (pow2 p1 <= n && n < pow2 (p1 + 1) &&
+		  pow2 p2 <= n && n < pow2 (p2 + 1)))
+	(ensures (p1 = p2))
+let pow2_interval_unique n p1 p2 =
+  if p1 > p2 
+  then Math.Lemmas.pow2_le_compat (p1 - 1) p2
+  else if p1 < p2
+  then Math.Lemmas.pow2_le_compat (p2 - 1) p1
+  else ()
+
+val pow2_floor_inv:
+  p:nat -> n:nat{pow2 p <= n && n < pow2 (p + 1)} ->
+  Lemma (pow2_floor n = p)
+let rec pow2_floor_inv p n =
+  pow2_interval_unique n (pow2_floor n) p
+
+val pow2_floor_pow2_pow2:
+  p:nat -> q:nat{p > q} ->
+  Lemma (pow2_floor (pow2 p + pow2 q) = p)
+let rec pow2_floor_pow2_pow2 p q =
+  Math.Lemmas.pow2_lt_compat p q;
+  pow2_floor_inv p (pow2 p + pow2 q)
+
+/// Invariants between internal roots and values
+
+val merkle_root_of_pow2:
+  #nelts:nat{is_pow2 nelts} -> vs:hash_seq{S.length vs = nelts} -> 
+  GTot hash
+let rec merkle_root_of_pow2 #nelts vs =
+  if nelts = 1 then S.index vs 0
+  else 
+    let lrt = merkle_root_of_pow2 #(nelts / 2) (S.slice vs 0 (nelts / 2)) in
+    let rrt = merkle_root_of_pow2 #(nelts / 2) (S.slice vs (nelts / 2) nelts) in
+    hash_from_hashes lrt rrt
+
+val num_iroots_of: nelts:nat -> GTot nat
+let rec num_iroots_of nelts =
+  if nelts = 0 then 0
+  else 1 + num_iroots_of (nelts - pow2 (pow2_floor nelts))
+
+val iroots_of_hashes:
+  nelts:nat -> 
+  hs:hash_seq{S.length hs = nelts} ->
+  GTot (iroots:hash_seq{S.length iroots = num_iroots_of nelts})
+let rec iroots_of_hashes nelts hs =
+  if nelts = 0 then hs
+  else S.cons (merkle_root_of_pow2 #(pow2 (pow2_floor nelts))
+				   (S.slice hs 0 (pow2 (pow2_floor nelts))))
+	      (iroots_of_hashes (nelts - (pow2 (pow2_floor nelts)))
+				(S.slice hs (pow2 (pow2_floor nelts)) nelts))
+
+unfold val iroots_of: 
+  nelts:nat -> es:elem_seq{S.length es = nelts} -> GTot hash_seq
+unfold let iroots_of nelts vs =
+  iroots_of_hashes nelts (seq_map hash_from_elem vs)
+
+/// High-level Merkle tree data structure
+
+noeq type merkle_tree =
+| MT: nelts:nat{nelts > 0} -> 
+      // The value buffer will be resized when elements are added.
+      // Resizing mechanism will be similar to that of C++ vector.
+      values:elem_seq{S.length values = nelts} ->
+      // The actual number of internal roots should be equal to 
+      // the number of "set" bits of `nelts`.
+      iroots:hash_seq{S.length iroots = num_iroots_of nelts} ->
+      merkle_tree
+
+/// Well-formedness
+
+unfold val merkle_tree_elems_wf:
+  nelts:nat{nelts > 0} -> 
+  values:elem_seq{S.length values = nelts} ->
+  iroots:hash_seq{S.length iroots = num_iroots_of nelts} ->
+  GTot bool
+unfold let merkle_tree_elems_wf nelts values iroots =
+  iroots_of nelts values = iroots
+
+unfold val merkle_tree_wf: merkle_tree -> GTot bool
+unfold let merkle_tree_wf mt =
+  merkle_tree_elems_wf (MT?.nelts mt) (MT?.values mt) (MT?.iroots mt)
+
+type wf_merkle_tree = mt:merkle_tree{merkle_tree_wf mt}
+
+/// Initialization
+
+val create_merkle_tree: unit -> wf_merkle_tree
+let create_merkle_tree _ = 
+  S.lemma_eq_elim (iroots_of 1 (S.create 1 elem_init))
+  		  (S.create 1 (hash_from_elem elem_init));
+  MT 1 (S.create 1 elem_init) (S.create 1 (hash_from_elem elem_init))
+
+/// Insertion
+
+unfold val insert_nelts: nat -> GTot nat
+unfold let insert_nelts nelts =
+  nelts + 1
+
+val insert_values: elem_seq -> elem -> GTot elem_seq
+let insert_values vs nv = 
+  S.append vs (S.create 1 nv)
+
+// val merge_iroots_seq:
+//   sz1:nat -> nelts1:nat{nelts1 = pow2 sz1 && nelts1 < pow2 max_nelts_sz - 1} ->
+//   irs1:hash_seq{S.length irs1 = num_iroots_of max_nelts_sz nelts1} ->
+//   sz2:nat{sz1 >= sz2} -> nelts2:nat{nelts2 = pow2 sz2 && nelts1 + nelts2 < pow2 max_nelts_sz - 1} ->
+//   irs2:hash_seq{S.length irs2 = num_iroots_of max_nelts_sz nelts2} ->
+//   GTot (mirs:hash_seq{S.length mirs = num_iroots_of max_nelts_sz (nelts1 + nelts2)})
+// let merge_iroots_seq sz1 nelts1 irs1 sz2 nelts2 irs2 =
+//   if sz1 = sz2 
+//   then S.create 1 (hash_from_hashes (S.index irs1 0) (S.index irs2 0))
+//   else (pow2_floor_pow2_pow2 sz1 sz2;
+//        assert (num_iroots_of max_nelts_sz nelts1 = 1);
+//        assert (num_iroots_of max_nelts_sz nelts2 = 1);
+//        assert (num_iroots_of max_nelts_sz (nelts1 + nelts2) =
+//        	      1 + num_iroots_of (max_nelts_sz - 1) (nelts1 + nelts2 - pow2 (pow2_floor (nelts1 + nelts2))));
+//        assert (num_iroots_of max_nelts_sz (nelts1 + nelts2) = 2);
+//        S.append irs1 irs2)
+
+val insert_iroots:
+  nelts:nat{nelts > 0} ->
+  irs:hash_seq{S.length irs = num_iroots_of nelts} ->
+  nh:hash ->
+  GTot (iirs:hash_seq{S.length iirs = num_iroots_of (insert_nelts nelts)})
+let rec insert_iroots nelts irs nh =
+  admit ()
+
+val insert: mt:wf_merkle_tree -> e:elem -> GTot wf_merkle_tree
+let insert mt e =
+  let nnelts = insert_nelts (MT?.nelts mt) in
+  let niroots = insert_iroots (MT?.nelts mt) (MT?.iroots mt) (hash_from_elem e) in
+  let nvalues = insert_values (MT?.values mt) e in
+  admit () // MT nnelts nvalues niroots
+
+/// Getting the Merkle root
+
+val padding_to_pow2:
+  nelts:nat{nelts > 0} -> GTot (sz:nat{
+    if nelts = 1 then sz = 0
+    else sz > 0 && pow2 (sz - 1) < nelts && nelts <= pow2 sz})
+let rec padding_to_pow2 nelts =
+  if nelts = 1 then 0
+  else if nelts % 2 = 0 then 1 + padding_to_pow2 (nelts / 2)
+  else 1 + padding_to_pow2 ((nelts + 1) / 2)
+
+val pad_hashes_pow2:
+  vs:hash_seq{S.length vs > 0} -> 
+  GTot (pvs:hash_seq{
+    S.length pvs = pow2 (padding_to_pow2 (S.length vs)) && 
+    S.slice pvs 0 (S.length vs) = vs})
+let pad_hashes_pow2 vs =
+  let pad = S.create (pow2 (padding_to_pow2 (S.length vs)) - S.length vs) hash_init in
+  S.append_slices vs pad;
+  S.append vs pad
+
+val merkle_root_of_hashes: vs:hash_seq{S.length vs > 0} -> GTot hash
+let merkle_root_of_hashes vs =
+  merkle_root_of_pow2 #(pow2 (padding_to_pow2 (S.length vs))) 
+		      (pad_hashes_pow2 vs)
+
+val merkle_root_of_iroots':
+  acc:hash -> irs:hash_seq -> GTot hash (decreases (S.length irs))
+let rec merkle_root_of_iroots' acc irs =
+  if S.length irs = 0 then acc
+  else merkle_root_of_iroots'
+       (hash_from_hashes (S.index irs (S.length irs - 1)) acc)
+       (S.tail irs)
+
+val merkle_root_of_iroots: irs:hash_seq -> GTot hash
+let rec merkle_root_of_iroots irs =
+  merkle_root_of_iroots' hash_init irs
+
+val merkle_root_of_iroots_ok:
+  mt:wf_merkle_tree ->
+  Lemma (merkle_root_of_iroots (MT?.iroots mt) =
+	merkle_root_of_hashes (seq_map hash_from_elem (MT?.values mt)))
+let merkle_root_of_iroots_ok mt =
+  admit ()
+
